

Interview Questions

Question 1. (Exercises 1.2) We stated, without proof, that the central pressure of the constant density star was a lower limit (§1.4); that is, central pressures must exceed $P_c = 3G\mathcal{M}^2/(8\pi\mathcal{R}^4)$. The proof of that statement requires a bit more work than we wish to attempt now. There is, however, a weaker lower limit on P_c . To get at this consider the function

$$f(r) = P(r) + \frac{G\mathcal{M}_r^2}{8\pi r^4}.$$

- 1) Show that $f(r)$ decreases outward with increasing r . (Hint: Differentiate $f(r)$ with respect to r and use the equation of hydrostatic equilibrium to show $df/dr < 0$.)
- 2) Assuming zero pressure at \mathcal{R} , demonstrate (almost immediately) that

$$P_c > \frac{G\mathcal{M}^2}{8\pi\mathcal{R}^4}$$

which is less stringent than that given by (1.42). Note that you must show \mathcal{M}_r^2/r^4 goes to zero as $r \rightarrow 0$.

- 1) Take the derivate of $f(r)$ respect to r :

$$\frac{df(r)}{dr} = \frac{dP(r)}{dr} + \frac{d}{dr} \left(\frac{G\mathcal{M}_r^2}{8\pi r^4} \right). \quad (1)$$

The equation of hydrostatic equilibrium (1.6) gives:

$$\frac{dP}{dr} = -\frac{G\mathcal{M}_r}{r^2}\rho.$$

We know that $d\mathcal{M}_r = 4\pi r^2 \rho(r) dr$, then using the chain rule, the second term in Equation 1 becomes:

$$\begin{aligned} \frac{d}{dr} \left(\frac{G\mathcal{M}_r^2}{8\pi r^4} \right) &= \frac{G}{8\pi} \frac{d}{dr} \left(\frac{\mathcal{M}_r^2}{r^4} \right) \\ &= \frac{G}{8\pi} \left[\frac{1}{r^4} \frac{d\mathcal{M}_r^2}{dr} + \mathcal{M}_r^2 \frac{d}{dr} \left(\frac{1}{r^4} \right) \right] \\ &= \frac{G}{8\pi} \left[\frac{1}{r^4} 2\mathcal{M}_r \frac{d\mathcal{M}_r}{dr} + \mathcal{M}_r^2 (-4) \frac{1}{r^5} \right] \\ &= \frac{G}{8\pi} \left[\frac{1}{r^4} 2\mathcal{M}_r 4\pi r^2 \rho - 4\mathcal{M}_r^2 \frac{1}{r^5} \right] \\ &= \frac{G\mathcal{M}_r}{r^2} \rho - \frac{G\mathcal{M}_r^2}{2\pi r^5}. \end{aligned}$$

Substitute the results of dP/dr and $d \left(\frac{G\mathcal{M}_r^2}{8\pi r^4} \right) / dr$ back to Equation 1:

$$\frac{df(r)}{dr} = -\frac{G\mathcal{M}_r}{r^2} \rho + \frac{G\mathcal{M}_r}{r^2} \rho - \frac{G\mathcal{M}_r^2}{2\pi r^5} = -\frac{G\mathcal{M}_r^2}{2\pi r^5}. \quad (2)$$

Since $G, \mathcal{M}_r, 2\pi > 0$, and we want $r > 0$ otherwise if $r = 0$ will blow up the equation,

$$\frac{G\mathcal{M}_r^2}{2\pi r^5} > 0;$$

thus, $df/dr < 0$.

2) Assuming zero pressure at \mathcal{R} : $P(\mathcal{R}) = 0$, then

$$f(\mathcal{R}) = P(\mathcal{R}) + \frac{G\mathcal{M}_r^2}{8\pi\mathcal{R}^4} = \frac{G\mathcal{M}_r^2}{8\pi\mathcal{R}^4}. \quad (3)$$

Note that, Equation (1.42) in the textbook is the result with the constant-density model. Then, as $r \rightarrow 0$, using Equation (1.41) in the textbook, $f(r)$ becomes:

$$\begin{aligned} \lim_{r \rightarrow 0} f(r) &= \lim_{r \rightarrow 0} \left[P(r) + \frac{G\mathcal{M}_r^2}{8\pi r^4} \right] \\ &= \lim_{r \rightarrow 0} P_c \left(1 - \frac{r^2}{\mathcal{R}^2} \right) + \frac{G}{8\pi} \lim_{r \rightarrow 0} \frac{\mathcal{M}_r^2}{r^4}, \end{aligned}$$

where the second term, by the constant-density model, $\mathcal{M}_r = r^3\mathcal{M}/\mathcal{R}^3$, is

$$\begin{aligned} \lim_{r \rightarrow 0} \frac{\mathcal{M}_r^2}{r^4} &= \lim_{r \rightarrow 0} \left(\frac{r^3}{\mathcal{R}^3} \mathcal{M} \right)^2 \frac{1}{r^4} \\ &= \frac{\mathcal{M}^2}{\mathcal{R}^6} \lim_{r \rightarrow 0} r^2 = 0. \end{aligned}$$

Therefore, $\lim_{r \rightarrow 0} f(r) = P_c$. Since $df/dr < 0$ as we shown in part 1, that means the function $f(r)$ is decreasing as r increasing. So,

$$\lim_{r \rightarrow 0} f(r) > f(\mathcal{R}) \implies P_c > \frac{G\mathcal{M}_r^2}{8\pi\mathcal{R}^4}, \quad (4)$$

as stated in the question.

Question 2. (Exercises 1.8) In the paragraph following the expression of the virial theorem (1.18) we stated that an extra term $-3P_S V_S$ should appear on the righthand side if we had chosen to consider only that part of the spherical star interior to $r = r_S$ having a volume V_S and a surface pressure P_S at r_S .

1) Prove this for the case of hydrostatic equilibrium; that is, show that the correct expression is

$$2K + \Omega - 3P_S V_S = 0.$$

Hint: Integrate (1.22) by parts using the equation of hydrostatic equilibrium (1.5 or 1.16) and the mass equation, and remember to only go out to r_S in that integration and the one for Ω (1.7).

2) Show explicitly that this amended version works for the constant density sphere.

1) Following by the hint, but using Equation (1.21) instead of (1.22), we have

$$\begin{aligned} 2K &= 3 \int_{r=0}^{r=r_S} P dV = 3 \left[(P_S V_S - P_0 V_0) - \int_P V dP \right] \\ &= 3P_S V_S - 3 \int_P V dP. \end{aligned} \quad (5)$$

Using Equation (1.16), the second term in Equation 5 becomes

$$\begin{aligned}
 3 \int_P V dP &= 3 \int_{\mathcal{M}} V \left(-\frac{G\mathcal{M}_r}{4\pi r^4} d\mathcal{M}_r \right) \\
 &= -3 \int_{\mathcal{M}} \left(\frac{4}{3}\pi r^3 \right) \left(\frac{G\mathcal{M}_r}{4\pi r^4} \right) d\mathcal{M}_r \\
 &= - \int_{\mathcal{M}} \frac{G\mathcal{M}_r}{r} d\mathcal{M}_r = \Omega.
 \end{aligned} \tag{6}$$

Then,

$$2K = 3P_S V_S - \Omega \implies 2K + \Omega - 3P_S V_S = 0,$$

as required by the question.

- 2) With the assumption of constant density sphere, we can directly calculate $2K$ and Ω . Since the density is unchanged in r dimension, we have \mathcal{M}_r :

$$d\mathcal{M}_r = 4\pi r^2 \rho dr \implies \mathcal{M}_r = \frac{4}{3}\pi \rho r^3.$$

We can find $P(r)$ from the equation of hydrostatic equilibrium,

$$\frac{dP}{dr} = -\frac{G\mathcal{M}_r}{r^2} \rho = -\frac{4\pi}{3} G \rho^2 r. \tag{7}$$

Take the integration on both side, we have

$$P(r) = -\frac{2\pi}{3} G \rho^2 r^2 + \text{const.}, \tag{8}$$

with the assumption that $P(r_S) = P_S$,

$$\begin{aligned}
 P(r_S) &= P_S = -\frac{2\pi}{3} G \rho^2 r_S^2 + \text{const.} \\
 \implies \text{const.} &= P_S + \frac{2\pi}{3} G \rho^2 r_S^2.
 \end{aligned}$$

Thus, Equation 8 is

$$P(r) = P_s + \frac{2\pi}{3} G \rho^2 (r_S^2 - r^2). \tag{9}$$

Note that $dV = d(4\pi r^3/3)$, then $2K$ is

$$\begin{aligned}
 2K &= \int_V P dV = 3 \int_0^{r_S} \left[\frac{2\pi}{3} G \rho^2 (r_S^2 - r^2) + P_S \right] d \left(\frac{4}{3}\pi r^3 \right) \\
 &= 3 \int_0^{r_S} \left[\frac{2\pi}{3} G \rho^2 (r_S^2 - r^2) + P_S \right] 4\pi r^2 dr \\
 &= 3 \left[\int_0^{r_S} \frac{2\pi}{3} G \rho^2 (r_S^2 - r^2) 4\pi r^2 dr + P_S \int_0^{r_S} 4\pi r^2 dr \right] \\
 &= \frac{16\pi^2}{15} G \rho^2 r_S^5 + 3P_S V_S.
 \end{aligned} \tag{10}$$

The Ω , by Equation 6, in this situation, is

$$\begin{aligned}
 \Omega &= 3 \int_P V dP = 3 \int_0^{r_S} \left(\frac{4}{3} \pi r^3 \right) \left(-\frac{4\pi}{3} G \rho^2 r dr \right) \\
 &= -3 \int_0^{r_S} \frac{16}{9} \pi^2 G \rho^2 r^4 dr \\
 &= -\frac{16\pi^2}{15} G \rho^2 r_S^5.
 \end{aligned} \tag{11}$$

Now,

$$2K + \Omega - 3P_S V_S = \frac{16\pi^2}{15} G \rho^2 r_S^5 + 3P_S V_S - \frac{16\pi^2}{15} G \rho^2 r_S^5 - 3P_S V_S = 0, \tag{12}$$

which the equation still holds for the constant density sphere.

END OF THE ASSIGNMENT